\begin{align}
 f(x)=\sqrt{x^2+z^2}-\sqrt{\left(x+\delta\right)^2+z^2}
\end{align}
\begin{align}
 \lim_{x \to 0} f(x)
 &= \lim_{x \to 0} \sqrt{x^2+z^2}-\sqrt{\left(x+\delta\right)^2+z^2} \\
 &= z-\sqrt{\delta^2+z^2}
\end{align}

For $\delta \ll z$, the limit is $0$.

\begin{align}
 \lim_{x \to \infty}f(x)
 &=\lim_{x \to \infty}\sqrt{x^2+z^2}-\sqrt{(x+\delta)^2+z^2} \\
 &= \lim_{x \to \infty}\frac{\left(\sqrt{x^2+z^2}-\sqrt{\left(x+\delta\right)^2+z^2}\right)\left(\sqrt{x^2+z^2}+\sqrt{\left(x+\delta\right)^2+z^2}\right)}
 {\sqrt{x^2+z^2}+\sqrt{\left(x+\delta\right)^2+z^2}}\\
 &= \lim_{x \to \infty}\frac{-2\delta}
 {\sqrt{x^2+z^2}+\sqrt{\left(x+\delta\right)^2+z^2}}\\
 &=\lim_{x \to \infty}\frac{x}{|x|}\frac{-\frac{\delta^2}{x}-2\delta}
 {\sqrt{1+\frac{z^2}{x^2}}+\sqrt{1+\frac{z^2}{x^2}+\frac{2\delta}{x}+\frac{\delta^2}{x^2}}}\\
 &=\frac{-2\delta}{\sqrt{1}+\sqrt{1}}\\
 &=-\delta
\end{align}

